Code cleanup: moved lemmas to pure etc, deleted many SearchAbouts, replaced FORALL by Forall_tl etc

HMAC_equivalence.v
@@ -2,36 +2,28 @@ Require Import Coqlib.
 Require Import Bvector.
 Require Import List.
 Require Import BinNums.
-(*Require Import Arith.
-Require Import HMAC_spec_list.*)
+(*Require Import Arith.*)
+Require Import common_lemmas.
 Require Import HMAC_functional_prog.
 Require Import ByteBitRelations.
+Require Import hmac_pure_lemmas.
 Require Import HMAC_common_defs.
 Require Import HMAC_common_lemmas.
+Require Import HMAC_spec_list.
 Require Import HMAC_spec_abstract.
-Require Import common_lemmas.
 
-Require Import BinNums.
 
-Lemma sha_h_length iv blk: length iv = c -> length blk = b ->
-      length (sha_h iv blk) = c.
-Proof. intros.
- unfold sha_h, intsToBits.
-  rewrite bytesToBits_len, pure_lemmas.length_intlist_to_Zlist.
-  rewrite common_lemmas.length_hash_block. reflexivity.
-  unfold bitsToInts. erewrite pure_lemmas.length_Zlist_to_intlist. reflexivity. 
-  erewrite bitsToBytes_len_gen. reflexivity.
-  rewrite H; reflexivity.
-  unfold bitsToInts. erewrite pure_lemmas.length_Zlist_to_intlist. reflexivity. 
-  erewrite bitsToBytes_len_gen. reflexivity.
-  rewrite H0; reflexivity.
-Qed.
-
-(*Duplicates the definition in Blist.v - could eliminate this once after merging with FCF*)
+(*Duplicates the definition in Blist.v - could eliminate this after merging with FCF*)
 Definition of_list_length (A : Set)(m : nat)(ls : list A)(pf : length ls = m) : Vector.t A m :=
   match pf with
     | eq_refl => Vector.of_list ls
   end. 
+
+Lemma of_length_proof_irrel n a: forall M, 
+      Vector.to_list (of_list_length bool n a M) = a.
+Proof. intros.
+  unfold of_list_length. destruct M. apply Vector.to_list_of_list_opp. 
+Qed.
 
 Section EQUIV.
 
@@ -92,12 +84,6 @@ Proof. intros. unfold fpad_v, of_list_length.
   subst; reflexivity.
 Qed.
 
-Require Import HMAC_spec_list.
-Definition Forall_tl (A : Type) (P : A -> Prop) (a : A) (l : list A) (H : Forall P (a :: l)):
-      Forall P l.
-inversion H. assumption.
-Defined. (*This is an alternative to FORALL that works better in the proofs below*)
-
 Fixpoint splitAndPad_aux (m:list Blist) (M: Forall (fun x => length x = 512%nat) m): 
            list (Bvector b) :=
 (match m as l return (Forall (fun x => length x = 512%nat) l) -> list (Bvector b) with
@@ -106,41 +92,11 @@ Fixpoint splitAndPad_aux (m:list Blist) (M: Forall (fun x => length x = 512%nat)
                     (splitAndPad_aux t (Forall_tl _ _ _ _ F))
  end) M.
 
-Lemma splitAndPad_aux_consD: forall h t M, splitAndPad_aux (cons h t) M =
-        cons (of_list_length _ _ h (Forall_inv M)) 
-                    (splitAndPad_aux t (Forall_tl _ _ _ _ M)).
-Proof. reflexivity. Qed.   
-Lemma splitAndPad_aux_cons_elim: forall h t M, exists pf1, exists pf2,
-      splitAndPad_aux (cons h t) M =
-        cons (of_list_length _ _ h pf1) (splitAndPad_aux t pf2).
-Proof. intros. exists (Forall_inv M). exists (Forall_tl _ _ _ _ M). reflexivity. Qed.
-
-Lemma splitAndPad_aux_cons_elim': forall h t M, 
-      splitAndPad_aux (cons h t) M =
-        cons (of_list_length _ _ h (Forall_inv M)) (splitAndPad_aux t (Forall_tl _ _ _ _ M)).
-Proof. reflexivity. Qed.
-
-
-Lemma  splitAndPad_aux_cons_intro: forall h t pf1 pf2, exists M,
-      splitAndPad_aux (cons h t) M =
-        cons (of_list_length _ _ h pf1) (splitAndPad_aux t pf2).
-Proof. intros. 
-  exists (Forall_cons _ pf1 pf2). rewrite splitAndPad_aux_cons_elim'. simpl.
-  reflexivity. (*This proof does not work for FORALL instead of forall_tl*)
-Qed.
-
-(*Definition splitAndPad_aux (m:list Blist) (M: Forall (fun x => length x = 512%nat) m): 
-           list (Bvector b).
-  induction m. apply nil.
-  apply (cons (of_list_length _ _ _ (Forall_inv M)) (IHm (FORALL _ _ _ _ M))).
-Defined.
-*)
-
-Lemma of_length_proof_irrel n a: forall M, 
-      Vector.to_list (of_list_length bool n a M) = a.
-Proof. intros.
-  unfold of_list_length. destruct M. apply Vector.to_list_of_list_opp. 
-Qed.
+Lemma splitAndPad_aux_consD h t M: 
+      splitAndPad_aux (cons h t) M
+      = (of_list_length _ _ h (Forall_inv M)) 
+         :: (splitAndPad_aux t (Forall_tl _ _ _ _ M)).
+Proof. reflexivity. Qed. 
 
 Lemma splitAndPad_aux_nil m M: m=nil -> splitAndPad_aux m M= nil.
 Proof. intros; subst. reflexivity. Qed.
@@ -150,13 +106,10 @@ Definition splitAndPad_v (m: Blist): list (Bvector b).
   apply InBlocks_Forall_512. apply sha_splitandpad_inc_InBlocks.
 Defined.
 
-Lemma splitAndPad_nil: (*exists blk, *) exists pf,
+Lemma splitAndPad_nil: exists pf,
   splitAndPad_v nil = 
   cons (of_list_length bool 512 (sha_splitandpad_inc nil) pf) nil. 
-(*cons blk nil /\
-   exists pf, exists xx, blk = of_list_length bool 512 xx pf*)
 Proof. unfold splitAndPad_v. 
-(*  unfold splitAndPad_aux. simpl.*)
   remember (InBlocks_Forall_512 (sha_splitandpad_inc_InBlocks nil)). clear Heqf.
   remember (toBlocks (sha_splitandpad_inc nil)).
   rewrite toBlocks_equation in Heql.
@@ -167,19 +120,14 @@ Proof. unfold splitAndPad_v.
       rewrite <- Heqm; trivial.
     simpl in H; clear Heqm. omega.
   rewrite leb_correct_conv in Heql.
-    Focus 2. rewrite Heqm; simpl; omega.
+    2: rewrite Heqm; simpl; omega.
   rewrite firstn_same in Heql.
-    Focus 2. rewrite Heqm; simpl; omega.
-  rewrite pure_lemmas.skipn_short in Heql.
-    Focus 2. rewrite Heqm; simpl; omega.
+    2: rewrite Heqm; simpl; omega.
+  rewrite skipn_short in Heql.
+    2: rewrite Heqm; simpl; omega.
   rewrite toBlocks_equation in Heql. subst l.
   simpl. eexists. reflexivity.
 Qed.
-
-Lemma  splitAndPad_aux_cons_intro': forall l h t (L: l = cons h t) pf1 pf2, exists M,
-      splitAndPad_aux l M =
-        cons (of_list_length _ _ h pf1) (splitAndPad_aux t pf2).
-Proof. intros. subst l. apply splitAndPad_aux_cons_intro. Qed.
 
 Lemma length_splitandpad_inner_aux: forall ssm pf,
   Forall2
@@ -198,7 +146,7 @@ Proof.
            rewrite firstn_length in pf.
            symmetry in Heqd. apply leb_complete in Heqd. 
            eapply NPeano.Nat.min_l_iff in pf. omega.
-    rewrite splitAndPad_aux_cons_elim'.
+    rewrite splitAndPad_aux_consD.
     constructor.
       rewrite of_length_proof_irrel. trivial.
     eapply (IHl (skipn 512 (b :: ssm))).
