Makefile
@@ -4,10 +4,8 @@ coqc Coqlib.v Integers.v SHA256.v ;
 coqc Axioms.v Extensionality.v Coqlib2.v common_lemmas.v functional_prog.v ;
 coqc XorCorrespondence.v # Takes a long time, skip after compiling once
 
-coqc pure_lemmas.v sha_padding_lemmas.v hmac_pure_lemmas.v ;
+coqc pure_lemmas.v hmac_pure_lemmas.v sha_padding_lemmas.v;
 coqc HMAC_functional_prog.v HMAC_functional_prog_Z.v HMAC_common_lemmas.v ;
 coqc Bruteforce.v ByteBitRelations.v ; # ByteBitRelations also takes a while
-coqc HMAC_common_defs.v HMAC_spec_pad.v HMAC_spec_concat.v HMAC_spec_list.v
-     HMAC_spec_abstract.v HMAC_equivalence.v
-
-
+coqc HMAC_common_defs.v HMAC_spec_pad.v HMAC_spec_concat.v HMAC_spec_list.v ;
+coqc HMAC_spec_abstract.v HMAC_equivalence.v
